changing to set-set-fact environments

LambdaTR.v
@@ -1,10 +1,4 @@
 
-(* Formalization of the core calculi found in
-   "Logical Types for Untyped Languages" 
-
-   -Andrew Kent *)
-
-Require Import TRLogic.
 
 Require Import LibTactics.
 Require Import List.
@@ -32,8 +26,6 @@ Hint Resolve id_eqdec.
 Definition id_eq (x y : id) : bool :=
 if id_eqdec x y then true else false.
 
-Definition X : id := (Id 0).
-
 (* Path Elements (accessors) *)
 Inductive acc : Type := car | cdr.
 
@@ -45,228 +37,76 @@ Hint Resolve acc_eqdec.
 Definition acc_eq (x y : acc) : bool :=
 if acc_eqdec x y then true else false.
 
-Definition π := list acc.
+Definition path := list acc.
 
 Hint Resolve list_eq_dec.
-Theorem π_eqdec : forall (x y: π),
+Theorem path_eqdec : forall (x y: path),
 {x = y} + {x <> y}.
 Proof. decide equality. Defined.
-Hint Resolve π_eqdec.
+Hint Resolve path_eqdec.
 
-Definition π_eq (x y : π) : bool :=
-if π_eqdec x y then true else false.
+Definition path_eq (x y : path) : bool :=
+if path_eqdec x y then true else false.
 
 (* Objects *)
 Inductive obj : Type :=
 | objnil : obj
-| objπ   : π -> id -> obj.
+| objπ : path -> id -> obj.
 
 Theorem obj_eqdec : forall (x y: obj),
 {x = y} + {x <> y}.
 Proof. decide equality. Defined.
-Hint Resolve obj_eqdec. 
+Hint Resolve obj_eqdec.
 
 Definition obj_eq (x y : obj) : bool :=
 if obj_eqdec x y then true else false.
 
 (* Types *)
-Inductive τ : Type :=
-| τT    : τ    (* Top *)
-| τN    : τ    (* Numbers *)
-| τt    : τ (* True *)
-| τf    : τ  (* False *)
-| τU    : list τ -> τ (* union *)
-| τλ    : id -> τ -> ψ -> ψ -> obj -> τ -> τ (* function *)
-| τcons : τ -> τ -> τ (* cons *)
+Inductive type : Type :=
+| tTop : type (* Top *)
+| tNum : type (* Numbers *)
+| tTrue : type (* True *)
+| tFalse : type (* False *)
+| tUnion : list type -> type (* union *)
+| tλ : id -> type -> env -> env -> obj -> type -> type (* function *)
+| tPair :  type -> type -> type (* cons pair *)
 
-with ψ : Type :=
-| ψfact : fact -> ψ
-| ψimpl : ψ -> ψ -> ψ
-| ψor   : ψ -> ψ -> ψ
-| ψand  : ψ -> ψ -> ψ
-| ψff   : ψ
-| ψtt   : ψ
+with env : Type :=
+| envNil   : env
+| envFalse : env -> env
+| envFact  : evidence -> env -> env
+| envOr    : env -> env -> env
 
-with fact : Type :=
-| fτ  : bool -> τ -> obj -> fact.
+with evidence : Type :=
+| fact : bool -> type -> obj -> evidence.
+Hint Constructors type env evidence.
 
 Hint Resolve bool_dec.
 
-Fixpoint τ_eqdec (x y : τ) : {x=y}+{x<>y}
-with ψ_eqdec (x y : ψ) : {x=y}+{x<>y}
-with fact_eqdec (x y : fact) : {x=y}+{x<>y}.
+Fixpoint type_eqdec (x y : type) : {x=y}+{x<>y}
+with env_eqdec (x y : env) : {x=y}+{x<>y}
+with evidence_eqdec (x y : evidence) : {x=y}+{x<>y}.
 Proof.
   decide equality.
   decide equality.
   decide equality.
 Defined.
+Hint Resolve type_eqdec env_eqdec evidence_eqdec.
 
-Hint Constructors τ ψ fact.
-Hint Resolve τ_eqdec ψ_eqdec fact_eqdec.
-
-(* Common Type Abbreviations *)
-Notation τB := (τU [τt ; τf]).
-Notation τ_ := (τU nil).
-
-Hint Resolve ψ_eqdec.
-
-Hint Resolve bool_dec.
-
-Definition τ_eq (x y : τ) : bool :=
-if τ_eqdec x y then true else false.
-
-Definition fact_eq (x y : τ) : bool :=
-if τ_eqdec x y then true else false.
-
-Definition ψ_eq (x y : ψ) : bool :=
-if ψ_eqdec x y then true else false.
-
-Inductive θ : Type :=
-| θfact : fact -> θ
-| θor   : θ -> θ -> θ
-| θand  : θ -> θ -> θ
-| θff   : θ
-| θtt   : θ.
-
-Definition negate_fact (f:fact) : fact :=
-match f with
-| fτ b t o => fτ (negb b) t o
-end.
-
-Fixpoint ψtoθ (prop:ψ) : θ :=
-match prop with
-| ψfact f   => θfact f
-| ψimpl p q => θor (notψtoθ p) (ψtoθ q)
-| ψor   p q => θor (ψtoθ p) (ψtoθ q)
-| ψand  p q => θand (ψtoθ p) (ψtoθ q)
-| ψff       => θff
-| ψtt       => θtt
-end
-
-with notψtoθ (prop:ψ) : θ :=
-match prop with
-| ψfact f   => θfact (negate_fact f)
-| ψimpl p q => θand (ψtoθ p) (notψtoθ q)
-| ψor   p q => θand (notψtoθ p) (notψtoθ q)
-| ψand  p q => θor (notψtoθ p) (notψtoθ q)
-| ψff       => θtt
-| ψtt       => θff
-end.
-
-Definition ψstoθs (ps:list ψ) : list θ :=
-map ψtoθ ps.
-
-Inductive Γ : Type :=
-| Γempty : Γ
-| Γfalse : Γ -> Γ
-| Γfact  : fact -> Γ -> Γ
-| Γor    : Γ -> Γ -> Γ.
-
-Fixpoint Γapp (Γ1 Γ2:Γ) : Γ :=
+Fixpoint env_app (Γ1 Γ2: env) : env :=
 match Γ1 with
-| Γempty => Γ2
-| Γfalse rest => Γfalse (Γapp rest Γ2)
-| Γfact f rest => Γfact f (Γapp rest Γ2)
-| Γor lhs rhs => Γor (Γapp lhs Γ2) (Γapp rhs Γ2)
+| envNil => Γ2
+| envFalse rest => envFalse (env_app rest Γ2)
+| envFact f rest => envFact f (env_app rest Γ2)
+| envOr lhs rhs => envOr (env_app lhs Γ2) (env_app rhs Γ2)
 end.
-
-Fixpoint θtoΓ (prop:θ) : Γ :=
-match prop with
-| θfact f  => Γfact f Γempty
-| θor p q  => Γor (θtoΓ p) (θtoΓ q)
-| θand p q => Γapp (θtoΓ p) (θtoΓ q)
-| θff      => Γfalse Γempty
-| θtt      => Γempty
-end.
-
-Fixpoint buildΓ' (props:list θ) : Γ :=
-match props with
-| nil => Γempty
-| p :: ps => Γapp (θtoΓ p) (buildΓ' ps)
-end.
-
-Definition buildΓ (ps:list ψ) := buildΓ' (ψstoθs ps).
-
-Inductive Proves : Γ -> fact -> Prop :=
-| P_Atom :
-    forall f E,
-      Proves (Γfact f E) f
-| P_False :
-    forall f E,
-      Proves (Γfalse E) f
-| P_Rest : 
-    forall f f' E,
-      Proves E f' ->
-      Proves (Γfact f E) f'
-| P_Or :
-    forall E1 E2 f,
-      Proves E1 f ->
-      Proves E2 f ->
-      Proves (Γor E1 E2) f.
-Hint Constructors Proves.
-
-Theorem Proves_dec : forall E f,
-{Proves E f} + {~Proves E f}.
-Proof.
-  induction E.
-  intros f. right.
-  intros contra; inversion contra.
-
-  intros f. left. apply P_False.
-
-  intros f'.
-  destruct (fact_eqdec f f'); subst.
-  left. apply P_Atom.
-  destruct (IHE f') as [Htrue | Hfalse].
-  left. apply P_Rest. assumption.
-  right. intros contra. inversion contra; subst. tryfalse. 
-  tryfalse. 
-
-  intros f.
-  destruct (IHE1 f); destruct (IHE2 f).
-  left. apply P_Or; auto.
-  right. intros contra; inversion contra; subst. tryfalse.
-  right. intros contra; inversion contra; subst. tryfalse.
-  right. intros contra; inversion contra; subst. tryfalse.
-Qed.
-
-(* 
-Proves Note!
-
-Although negation is included in this logic in some sense - deriving
-contradictions via the negation of facts is not.
-
-This behavior can be specifically included in expandΓ if desired.
-
-*)
-
-(* Option used so None can represent a false environment (i.e. ff is proven) *)
-Definition fact_in (f : fact) (fs : option (list fact)) : bool := 
-match fs with
-| None => true
-| Some facts =>
-  if in_dec fact_eqdec f facts then true else false
-end.
-
-Fixpoint expProves' (f:fact) (facts:list fact) (E:Γ) 
-         (expΓ: list fact -> option (list fact)) : bool :=
-match E with
-| Γempty => fact_in f (expΓ facts)
-| Γfalse rest => true
-| Γfact f rest => expProves' f (f :: facts) rest expΓ
-| Γor lhs rhs => andb (expProves' f facts lhs expΓ) (expProves' f facts rhs expΓ)
-end.
-
-Definition expProves (f:fact) (E:Γ) 
-           (expΓ: list fact -> option (list fact)): bool :=
-expProves' f nil E expΓ.
 
 
 (* Constant Operations *)
 Inductive c_op : Type :=
-| op_add1   : c_op
+| op_add1 : c_op
 | op_iszero : c_op
-| op_isnum  : c_op
+| op_isnum : c_op
 | op_isbool : c_op
 | op_isproc : c_op
 | op_iscons : c_op.
@@ -293,7 +133,7 @@ Definition p_op_eq (x y : p_op) : bool :=
 if p_op_eqdec x y then true else false.
 
 (* Primitive Operations *)
-Inductive primop : Type := 
+Inductive primop : Type :=
 | prim_c : c_op -> primop
 | prim_p : p_op -> primop.
 
@@ -306,100 +146,40 @@ Definition primop_eq (x y : primop) : bool :=
 if primop_eqdec x y then true else false.
 
 (* Expressions *)
-Inductive e : Type :=
-| e_var    : id -> e
-| e_app    : e -> e -> e
-| e_abs    : id -> τ -> e -> e
-| e_if     : e -> e -> e -> e
-| e_primop : primop -> e
-| e_true   : e
-| e_false  : e
-| e_num    : nat -> e
-| e_cons   : e -> e -> e
-| e_let    : id -> e -> e -> e.
+Inductive exp : Type :=
+| expVar : id -> exp
+| expApp : exp -> exp -> exp
+| expAbs : id -> type -> exp -> exp
+| expIf : exp -> exp -> exp -> exp
+| expPrimop : primop -> exp
+| expT : exp
+| expF : exp
+| expNum : nat -> exp
+| expCons : exp -> exp -> exp
+| expLet : id -> exp -> exp -> exp.
 
-Notation car' := (e_primop (prim_p op_car)).
-Notation cdr' := (e_primop (prim_p op_cdr)).
-Notation add1' := (e_primop (prim_c op_add1)).
-Notation iszero' := (e_primop (prim_c op_iszero)).
-Notation isnum' := (e_primop (prim_c op_isnum)).
-Notation isbool' := (e_primop (prim_c op_isbool)).
-Notation isproc' := (e_primop (prim_c op_isproc)).
-Notation iscons' := (e_primop (prim_c op_iscons)).
+Notation car' := (expPrimop (prim_p op_car)).
+Notation cdr' := (expPrimop (prim_p op_cdr)).
+Notation add1' := (expPrimop (prim_c op_add1)).
+Notation iszero' := (expPrimop (prim_c op_iszero)).
+Notation isnum' := (expPrimop (prim_c op_isnum)).
+Notation isbool' := (expPrimop (prim_c op_isbool)).
+Notation isproc' := (expPrimop (prim_c op_isproc)).
+Notation iscons' := (expPrimop (prim_c op_iscons)).
 
-Theorem e_eqdec : forall (x y : e),
+Theorem exp_eqdec : forall (x y : exp),
 {x = y} + {x <> y}.
 Proof. decide equality. Defined.
 
-Definition e_eq (x y : e) : bool :=
-if e_eqdec x y then true else false.
+Definition exp_eq (x y : exp) : bool :=
+if exp_eqdec x y then true else false.
 
-(* TODO: Do we need Integers to represent numbers? Reals? *)
-
-(* Environments *)
-Definition env := list ψ.
-
-Theorem env_eqdec : forall (x y : env),
-{x=y}+{x<>y}.
-Proof.
-  decide equality.
-Defined.
-
-Definition env_eq (x y : env) : bool :=
-if env_eqdec x y then true else false.
-
-Definition c_op_type (c : c_op) : τ :=
-match c with
-| op_isnum => 
-  (τλ X 
-         τT 
-         (ψfact (fτ true τN (objπ [] X))) 
-         (ψfact (fτ false τN (objπ [] X))) 
-         objnil 
-         τB)
-| op_isproc =>
-  (τλ X 
-         τT 
-         (ψfact (fτ true (τλ X τ_ ψtt ψff objnil τT) (objπ [] X))) 
-         (ψfact (fτ false (τλ X τ_ ψtt ψff objnil τT) (objπ [] X))) 
-         objnil 
-         τB)
-| op_isbool =>
-  (τλ X
-         τT
-         (ψfact (fτ true τB (objπ [] X)))
-         (ψfact (fτ false τB (objπ [] X)))
-         objnil
-         τB)
-| op_iscons =>
-  (τλ X
-         τT
-         (ψfact (fτ true (τcons τT τT) (objπ [] X)))
-         (ψfact (fτ false (τcons τT τT) (objπ [] X)))
-         objnil
-         τB)
-| op_add1 =>
-  (τλ X
-      τN
-      ψtt
-      ψtt
-      objnil
-      τN)
-| op_iszero =>
-  (τλ X
-      τN
-      ψtt
-      ψtt
-      objnil
-      τB)
-end.
-
-Fixpoint setU {X:Type} (dec : forall x y : X, {x=y} + {x<>y}) 
+Fixpoint setU {X:Type} (dec : forall x y : X, {x=y} + {x<>y})
                        (l:list (set X)) : set X :=
 match l with
 | nil => nil
 | x :: xs => set_union dec x (setU dec xs)
-end. 
+end.
 
 (* free variables in objects *)
 Definition fv_set_o (o : obj) : set id :=
@@ -410,45 +190,43 @@ end.
 
 (* free variables in types *)
 
-Fixpoint fv_set_t (t : τ) : set id :=
+Fixpoint fv_set_t (t : type) : set id :=
 match t with
-| τU l =>
-  fold_left (fun ids next => 
-               set_union id_eqdec 
-                         ids 
+| tUnion l =>
+  fold_left (fun ids next =>
+               set_union id_eqdec
+                         ids
                          (fv_set_t next))
             l
             nil
-| τλ x t1 p1 p2 o t2 =>
+| tλ x t1 p1 p2 o t2 =>
   setU id_eqdec
        [[x];
         (fv_set_t t1);
-        (fv_set_p p1);
-        (fv_set_p p2);
+        (fv_set_env p1);
+        (fv_set_env p2);
         (fv_set_o o);
         (fv_set_t t2)]
-| τcons t1 t2 => 
+| tPair t1 t2 =>
   set_union id_eqdec
-            (fv_set_t t1) 
+            (fv_set_t t1)
             (fv_set_t t2)
 | _ => nil
 end
 
-(* free variables in propositions *)
-with fv_set_p (p: ψ) : set id :=
-let fv_set_fact := ((fix fv_set_fact (f:fact) : set id:= 
-     match f with
-     | fτ b t o  => 
-       set_union id_eqdec (fv_set_o o) (fv_set_t t)
-     end)) in
-match p with
-| ψfact f => (fv_set_fact f)
-| ψimpl p q => set_union id_eqdec (fv_set_p p) (fv_set_p q)
-| ψor p q => set_union id_eqdec (fv_set_p p) (fv_set_p q)
-| ψand p q => set_union id_eqdec (fv_set_p p) (fv_set_p q)
-| _ => nil
-end.
+with fv_set_f (f:evidence) : set id :=
+match f with
+| fact b t o => set_union id_eqdec (fv_set_t t) (fv_set_o o)
+end
 
+(* free variables in the proposition environment*)
+with fv_set_env (E : env) : set id :=
+match E with
+| envNil => nil
+| envFalse rest => fv_set_env rest
+| envFact f rest => set_union id_eqdec  (fv_set_f f) (fv_set_env rest)
+| envOr lhs rhs => set_union id_eqdec (fv_set_env lhs) (fv_set_env rhs)
+end.
 
 Definition subst_o (o1 o2:obj) (x:id) : obj :=
 match o1 with
@@ -461,68 +239,51 @@ match o1 with
   end
 end.
 
-Inductive sign : Type := pos | neg.
-
-Definition sign_truth (p:sign) : ψ :=
-match p with
-| pos => ψtt
-| neg => ψff
-end.
-
-Definition sign_flip (p:sign) : sign :=
-match p with
-| pos => neg
-| neg => pos
-end.
-
 (* subst+ and - for properties*)
-Fixpoint subst_p (s : sign) 
-                 (p:ψ) 
-                 (o:obj) 
-                 (x:id) : ψ :=
-match p with
-| ψfact (fτ b t (objπ pth1 z)) =>
-  match id_eq x z , set_mem id_eqdec z (fv_set_t t) with
-  | true, _ => 
+Fixpoint subst_env (E:env)
+                   (o:obj)
+                   (x:id) : env :=
+match E with
+| envNil => envNil
+| envFalse rest => envFalse (subst_env rest o x)
+| envFact (fact fb ft (objπ pth1 z)) rest => 
+  match id_eq x z, set_mem id_eqdec z (fv_set_t ft) with
+  | true, _ =>
     match o with
-    | objnil => (sign_truth s)
-    | objπ pth2 y =>
-      ψfact (fτ b (subst_t s t o x) (objπ (pth1 ++ pth2) y))
+    | objnil => subst_env rest o x (* tt  - ignore *)
+    | objπ pth2 y  => 
+      envFact (fact fb (subst_t ft o x) (objπ (pth1 ++ pth2) y)) (subst_env rest o x)
     end
-  | false, false => p
-  | false, true => (sign_truth s)
-  end
-| ψimpl P Q => ψimpl (subst_p (sign_flip s) P o x) 
-                   (subst_p s Q o x)
-| ψor P Q => ψor (subst_p s P o x) (subst_p s Q o x)
-| ψand P Q => ψand (subst_p s P o x) (subst_p s Q o x)
-| _ => p
+  | false, false => envFact (fact fb ft (objπ pth1 z)) (subst_env rest o x)
+  | false, true => subst_env rest o x (* tt  - ignore *)
+  end 
+| envFact (fact fb ft objnil) rest => envFact (fact fb ft objnil) (subst_env rest o x)
+| envOr lhs rhs => envOr (subst_env lhs o x) (subst_env rhs o x)
 end
 
 (* type substitution *)
-with subst_t (s:sign) 
-             (t:τ) 
-             (o:obj) 
-             (x:id) : τ :=
+with subst_t (t:type)
+             (o:obj)
+             (x:id) : type :=
 match t with
-| τU l => τU (map (fun t' => subst_t s t' o x) l)
-| τλ y t1 p1 p2 o2 t2 =>
+| tUnion l => tUnion (map (fun t' => subst_t t' o x) l)
+| tλ y t1 p1 p2 o2 t2 =>
   if id_eq x y
   then t
-  else τλ y
-             (subst_t s t1 o x)
-             (subst_p s p1 o x)
-             (subst_p s p2 o x)
-             (subst_o o2 o x)
-             (subst_t s t2 o x)
-| τcons t1 t2 => τcons (subst_t s t1 o x) 
-                         (subst_t s t2 o x)
+  else tλ y
+          (subst_t t1 o x)
+          (subst_env p1 o x)
+          (subst_env p2 o x)
+          (subst_o o2 o x)
+          (subst_t t2 o x)
+| tPair t1 t2 => tPair (subst_t t1 o x)
+                       (subst_t t2 o x)
 | _ => t
 end.
 
 Inductive SubObj : relation obj :=
 | SO_Refl : forall x, SubObj x x
-| SO_Top  : forall x, SubObj x objnil.
+| SO_Top : forall x, SubObj x objnil.
 Hint Constructors SubObj.
 
 Theorem sub_obj : forall x y,
@@ -536,353 +297,140 @@ Proof.
   inversion contra; crush.
 Defined.
 
-(*
-Fixpoint contains_bottom (E:Γ) : bool :=
-match E with
-| nil => false
-| p :: ps => 
-  match p with
-  | T t pth y => if (type_eq t τ_)
-                 then true
-                 else contains_bottom ps
-  | _ => contains_bottom ps
-  end
+Definition fact_symbol (f:evidence) : option id :=
+match f with
+| fact b t (objπ pth x) => Some x
+| _ => None
 end.
 
-Definition in_Γ (p:prop) (E:Γ) := in_dec prop_eqdec p E.
-Definition ext_Γ (p:prop) (E:Γ) := set_add prop_eqdec p E.
-
-(* Creates a set of all properties which imply Q in the environment. *)
-Fixpoint implicators (E:Γ) (Q:prop) : set prop :=
-match E with
-| nil => []
-| p :: ps => 
-  match p with
-  | ψimp P Q' => if prop_eq Q Q' 
-                 then ext_Γ P (implicators ps Q)
-                 else implicators ps Q
-  | _ => implicators ps Q
-  end
-end.
+Fixpoint contains_false (E:env) : bool := false. (* TODO *)
 
 
-Program Fixpoint proves (E:Γ) (p:prop) {measure (prop_depth p)} : bool :=
-(* L-ATOM *)
-if in_Γ p E then true else
-(* L-τt *)
-if prop_eq τt p then true else
-(* L-τf *)
-if in_Γ τf E then true else
-(* L-BOT *)
-if contains_bottom E then true else
-(* L-IMPE *)
-if prove_any (implicators E p) then true else
-(* L-ORE *)
-if disj_proves 
-(* L-ANDE *)
+Inductive Proves : env -> fact -> Prop
+| P_Atom :
+    forall f E,
+      Proves (Γfact f E) f
+| P_False :
+    forall f E,
+      Proves (Γfalse E) f
+| P_Cons :
+    forall f f' E,
+      Proves E f' ->
+      Proves (Γfact f E) f'
+| P_Or :
+    forall E1 E2 f,
+      Proves E1 f ->
+      Proves E2 f ->
+      Proves (Γor E1 E2) f
+| P_Sub :
+    forall t σ E pth x,
+      Subtype t σ ->
+      Proves E (fτ true t (objπ pth x)) ->
+      Proves E (fτ true σ (objπ pth x))
+| P_SubNeg :
+    forall E t σ pth x,
+      Subtype t σ ->
+      Proves E (fτ false σ (objπ pth x)) ->
+      Proves E (fτ false t (objπ pth x))
+| P_Update :
+    forall E t1 pth1 x b σ pth2 t2,
+      Proves E (fτ true t1 (objπ pth1 x)) ->
+      Proves E (fτ b σ (objπ (pth2 ++ pth1) x)) ->
+      Update t1 (b, σ) pth2 t2 ->
+      Proves E (fτ b t2 (objπ pth1 x))
 
-(* 
-   OrE
-   check all disjuctions, test if adding either side to E proves the prop,
-   if both prove the prop, then it's proven because that disjunction is in there
-
-   AndE
-   check all conjuctions, test if adding either side to E proves the prop,
-   if either prove the prop, then it's proven because that conjunction is in there
-
-*)
-
-with disj_proves (E:Γ) (p:prop) : bool :=
-match E with
-| nil => false
-| q :: qs
-  match q with
-  | OR r s => if (andb (proves (r :: qs)) (proves (s :: qs)))
-              then true
-              else disj
-
-with prove_any (E:Γ) (s:set prop) : bool :=
-match s with
-| nil => false
-| p :: ps => if proves E p 
-             then true
-             else proves_any E ps
-end
-
-with subtype (x y: type) : bool := false
-
-with update (x: type) (s:sign) (y:type) (p:path) : type := τ_
-
-with restrict (x y: type) : type := τ_
-
-with remove (x y: type) : type := τ_.
-*)
-
-Definition isU (t:τ) : bool :=
-match t with
-| τU _ => true
-| _ => false
-end.
-
-Definition share_types (t1 t2:τ) : bool := true.
-
-(* BOOKMARK
-
-  I've merged the logic and lambda calc up till this point, just about
-  to look at how the SubType relation works with the above new defs.
- *)
-
-(* SubType *)
-Inductive SubType : relation τ :=
-| S_Refl : forall x, SubType x x
-| S_Top : forall x, SubType x τT
-| S_UnionSuper : 
-    forall t s,
-      (exists t', set_In t' s /\ SubType t t') ->
-      SubType t (τU s)
-| S_UnionSub :
-    forall t s,
-      (forall t', set_In t' s -> SubType t' t) ->
-      SubType (τU s) t
-| S_Fun : 
-    forall x t1 t2 p1 p2 o t1' t2' p1' p2' o',
-      SubType t1   t1' ->
-      SubType t2   t2' ->
-      Proves  [p1] p1' ->
-      Proves  [p2] p2' ->
-      SubObj  o    o'  ->
-      SubType (τλ x t1 p1 p2 o t2) 
-              (τλ x t1' p1' p2' o' t2')
-| S_Pair :
-    forall t1 t2 t1' t2',
-      SubType t1 t1' ->
-      SubType t2 t2' ->
-      SubType (τcons t1 t2) (τcons t1' t2')
-
-with Update : τ -> (bool * τ) -> π -> τ -> Prop :=
-| UP_Car : 
-    forall τ1 v pth σ1 updated,
-      Update τ1 v pth updated ->
-      Update (τcons τ1 σ1) v (pth ++ [car]) (τcons updated σ1)
-| UP_Cdr :
-    forall t1 b t2 pth t3 σ,
-      Update σ ( b , t2 ) pth t3 ->
-      Update (τcons t1 σ) (b, t2) (pth ++ [car]) (τcons t3 σ)
-
-| UP_T :
-    forall τ σ ε r,
-      Restrict τ σ r ->
-      Update τ (true, σ) ε r
-| UP_NT :
-    forall τ σ ε r,
-      Remove τ σ r ->
-      Update τ (false, σ) ε r
+with NotProves : env -> fact -> Prop
+| NP_Nil :
+    forall f E,
+      NotProves envNil f
+| NP_Cons :
+    forall f E x t',
+      contains_false E = false ->
+      NotProves E f ->
+      fact_symbol f = Some x -> (* TODO: Proving a fact with a null object...? *)
+      (* And for all things proven about x in E, neither they nore their updated type are super-types
+         of the type in this query, then it is not proven hear either *)
 
 
-with Restrict : τ -> τ -> τ -> Prop :=
-| RES_Bot : 
-      forall τ1 σ1,
-        share_types τ1 σ1 = false ->
-(*    forall τ1 ψ1 ψ1' o1 σ1 ψ2 ψ2' o2,
-      ~(exists v, (and (TypeOf [] v τ1 ψ1 ψ1' o1) 
-                       (TypeOf [] v σ1 ψ2 ψ2' o2))) -> 
-  This is a non positive usage of TypeOf.... *)
+with ProvesAll : env -> env -> Prop :=
+| PAll_empty :
+    forall E,
+      ProvesΓ E envNil
+| PAll_Cons :
+    forall E1 E2 f,
+      Proves E1 f ->
+      ProvesAll E1 E2 ->
+      ProvesAll E1 (Γfact f E2)
+| PΓ_Or_l :
+    forall E E1 E2,
+      ProvesAll E E1 ->
+      ProvesAll E (Γor E1 E2)
+| PΓ_Or_r :
+    forall E E1 E2,
+      ProvesΓ E E2 ->
+      ProvesΓ E (Γor E1 E2)
 
-      Restrict τ1 σ1 τ_
-| RES_U_nil :
-    forall σ1,
-      Restrict τ_ σ1 τ_
-| RES_U_cons :
-    forall τ1 τs σ1 r rs,
-      Restrict (τU τs) σ1 (τU rs) ->
-      Restrict τ1 σ1 r ->
-      Restrict (τU (τ1 :: τs)) σ1 (τU (r :: rs))
-| RES_Tsub :
-    forall τ1 σ1,
-      SubType τ1 σ1 ->
-      Restrict τ1 σ1 τ1
-| RES_other :
-    forall τ1 ψ1 ψ1' o1 σ1 ψ2 ψ2' o2,
-      share_types t1 σ1 = true ->
-      ~SubType τ1 σ1 ->
-      isU τ1 = false ->
-      Restrict τ1 σ1 σ1
-with Remove : τ -> τ -> τ -> Prop :=
-| REM_Bot :
-    forall τ1 σ1,
-      SubType τ1 σ1 ->
-      Remove τ1 σ1 τ_
-| REM_U_nil :
-    forall σ1,
-      Remove τ_ σ1 τ_
-| REM_U_cons :
-    forall τ1 τs σ1 r rs,
-      Remove (τU τs) σ1 (τU rs) ->
-      Remove τ1 σ1 r ->
-      Remove (τU (τ1 :: τs)) σ1 (τU (r :: rs))
-| REM_other :
-    forall σ1 τ1,
-      ~SubType τ1 σ1 ->
-      isU τ1 = false ->
-      Remove τ1 σ1 τ1
+with NotProvesAll : env -> env -> Prop :=
 
+with Subtype : type -> type -> Prop :=
 
-(* Typing Rules *)
+with NotSubtype : type -> type -> Prop :=
+
+with Update :
+
+with Restrict
+
+with Remove :
+
 with TypeOf : 
-  Γ -> e -> τ -> ψ -> ψ -> obj -> Prop :=
-| Τ_Num : 
-    forall E n, 
-      TypeOf E (e_num n) τN ψT ψF obj_nil
-| T_Const : 
-    forall E c,
-      TypeOf E 
-             (e_primop (prim_c c)) 
-             (c_op_type c) 
-             ψT 
-             ψF 
-             obj_nil
-| T_True :
-    forall E,
-      TypeOf E e_true τt ψT ψF obj_nil
-| T_False :
-    forall E,
-      TypeOf E e_false τf ψF ψT obj_nil
-| T_Var :
-    forall E x t,
-      In (ψτ true t [] x) E ->
-      TypeOf E 
-             (e_var x) 
-             t
-             (ψτ false τf [] x)
-             (ψτ true τf [] x)
-             (obj_p [] x)
-| T_Abs :
-   forall E s x e t pT pF o,
-     TypeOf ((ψτ true s [] x) :: E) e t pT pF o ->
-     TypeOf E 
-            (e_abs x s e) 
-            (τλ x s pT pF o t) 
-            ψT 
-            ψF 
-            obj_nil
-| T_App :
-   forall E e x s pTf pFf t pT pF of o e' pT' pF' o',
-     TypeOf E e (τλ x s pTf pFf of t) pT pF o ->
-     TypeOf E e' s pT' pF' o' ->
-     TypeOf E (e_app e e') 
-            (subst_t pos t o' x) 
-            (subst_p pos pTf o' x) 
-            (subst_p pos pFf o' x) 
-            (subst_o of o' x)
-| T_If :
-   forall E e1 t1 pT1 pF1 o1 e2 t pT2 pF2 o e3 pT3 pF3,
-     TypeOf E e1 t1 pT1 pF1 o1 ->
-     TypeOf (pT1 :: E) e2 t pT2 pF2 o ->
-     TypeOf (pF1 :: E) e3 t pT3 pF3 o ->
-     TypeOf E (e_if e1 e2 e3) t (ψor pT2 pT3) (ψor pF2 pF3) o 
-| T_Subsume :
-   forall E e t pT pF o pT' pF' t' o',
-     TypeOf E e t pT pF o ->
-     Proves (pT :: E) pT' ->
-     Proves (pF :: E) pF' ->
-     SubType t t' ->
-     SubObj o o' ->
-     TypeOf E e t' pT' pF' o'
-| T_Cons :
-   forall E e1 t1 p1 p1' o1 e2 t2 p2 p2' o2,
-     TypeOf E e1 t1 p1 p1' o1 ->
-     TypeOf E e2 t2 p2 p2' o2 ->
-     TypeOf E (e_cons e1 e2) (τcons t1 t2) ψT ψF obj_nil
-| T_Car :
-   forall E e t1 t2 p0 p0' o o' p p' x,
-     TypeOf E e (τcons t1 t2) p0 p0' o ->
-     p = (subst_p pos (ψτ false τf [car] x) o x) ->
-     p' = (subst_p pos (ψτ true τf [car] x) o x) ->
-     o' = subst_o (obj_p [car] x) o x ->
-     TypeOf E (e_app car' e) t1 p p' o'
-| T_Cdr :
-   forall E e t1 t2 p0 p0' o o' p p' x,
-     TypeOf E e (τcons t1 t2) p0 p0' o ->
-     p = (subst_p pos (ψτ false τf [cdr] x) o x) ->
-     p' = (subst_p pos (ψτ true τf [cdr] x) o x) ->
-     o' = subst_o (obj_p [cdr] x) o x ->
-     TypeOf E (e_app cdr' e) t2 p p' o'
-| T_Let :
-   forall E e0 t p0 p0' o0 e1 t' p1 p1' o1 x,
-   TypeOf E e0 t p0 p0' o0 ->
-   TypeOf ((ψτ true t [] x) ::
-           (ψimp (ψτ false τf [] x) p0) ::
-           (ψimp (ψτ true τf [] x) p0') :: 
-           E)
-          e1 
-          t' 
-          p1 
-          p1' 
-          o1 ->
-   TypeOf E 
-          (e_let x e0 e1) 
-          (subst_t pos t' o0 x)
-          (subst_p pos p1 o0 x)
-          (subst_p pos p1' o0 x)
-          (subst_o o1 o0 x).
 
 
-Scheme proves_mut := Induction for Proves Sort Prop
-with subtype_mut := Induction for SubType Sort Prop.
-
-Theorem false_dec : forall E,
-{Proves E τf} + {~Proves E τf}.
-Proof.
-  intros E; induction E.
-  right; intros contra.
-  inversion contra; subst. tryfalse.
-
-
-Fixpoint proves_dec (E: Γ) (p : prop) : {Proves E p} + {~Proves E p}
-with subtype_dec (x y: type) : {SubType x y} + {~SubType x y}.
-Proof.
-  clear provse_d
-  eauto.
-  
-  Check proves_mut.
-  eapply proves_mut.
-  generalize dependent E.
-  
-  apply proves_mut.
-  induction p; crush.
-  generalize dependent y.
-  induction x; crush.
-Defined.
-
-
-Theorem proves : forall E p,
-{Proves E p} + {~Proves E p}.
-Proof.
-  intros E. induction E as [| q E'].
-  intro p. destruct p.
-
-  (* (T t p i) *)
-  left. apply L_False.
-  right; intros contra. inversion contra; subst.
-  tryfalse. 
-
-  Lemma proves_nil_false_false :
-    ~ Proves [] τf.
-    Proof.
-      intros contra.
-      inversion contra; crush.
-
-inversion H; subst. tryfalse.
-
-  right. intros contra. inversion contra; subst. tryfalse.
-  right; intros contra.
-  inversion contra; subst. tryfalse.
-  inversion H. subst. tryfalse. subst.
- inversion contra; crush.
-  eauto.
-
-
-
-
+(*  TODO: Build this into the typing relation
+Definition c_op_type (c : c_op) : type :=
+match c with
+| op_isnum =>
+  (tλ X
+         tTrue
+         (envFact (fact true tNum (objπ [] X)) envEmpty)
+         (envFact (fact false tNum (objπ [] X)) envEmpty)
+         objnil
+         τB)
+| op_isproc =>
+  (tλ X
+         τT
+         (envFact (fact true (τλ X τ_ ψtt ψff objnil τT) (objπ [] X)) envEmpty)
+         (envFact (fact false (τλ X τ_ ψtt ψff objnil τT) (objπ [] X)) envEmpty)
+         objnil
+         τB)
+| op_isbool =>
+  (tλ X
+         τT
+         (envFact (fact true τB (objπ [] X)) envEmpty)
+         (envFact (fact false τB (objπ [] X)) envEmpty)
+         objnil
+         τB)
+| op_iscons =>
+  (tλ X
+         τT
+         (envFact (fτ true (τcons τT τT) (objπ [] X)) envEmpty)
+         (envFact (fτ false (τcons τT τT) (objπ [] X)) envEmpty)
+         objnil
+         τB)
+| op_add1 =>
+  (tλ X
+      τN
+      envEmpty
+      envEmpty
+      objnil
+      τN)
+| op_iszero =>
+  (tλ X
+      τN
+      envEmpty
+      envEmpty
+      objnil
+      τB)
+end.
+*)
 
 End LTR.
